wip wip

examples/low-level/crypto/Crypto.WIP.fst
@@ -471,6 +471,88 @@ let rec find_entry_blocks (#i:id) (#rgn:rid)
 			find_mac prf_entries x0 == Some (PRF.macRange rgn i x0 (Seq.index blocks 0).range)))
      = Crypto.AEAD.Lemmas.Part2.find_entry_blocks i rgn n entries prf_entries h //TODO: duplicate ... remove the indirection
 
+val counterblocks_contains_all_cipher_blocks:   
+  i:id{safeId i} ->
+  rgn:region -> 
+  x:PRF.domain i{PRF.ctr_0 i <^ ctr x} -> 
+  len:u32{len <> 0ul /\ safelen i (v len) (PRF.ctr_0 i +^ 1ul)} ->
+  remaining_len:u32{safelen i (v remaining_len) x.ctr /\ remaining_len <=^ len} -> 
+  plain:Crypto.Plain.plain i (v len) -> 
+  cipher:lbytes (v len) -> 
+  Lemma (requires (let completed_len = v len - v remaining_len in
+  		   let n_blocks = v x.ctr - v (offset i) in
+		   (completed_len = v len /\ n_blocks == num_blocks' i (v len)) \/
+		    completed_len = FStar.Mul (n_blocks * v (PRF.blocklen i))))
+        (ensures
+	    (let x0 = {x with ctr=ctr_0 i +^ 1ul} in
+	     let all_blocks = counterblocks i rgn x0 (v len) 0 (v len) plain cipher in
+	     let n_blocks = v x.ctr - v x0.ctr in
+	     n_blocks <= Seq.length all_blocks /\
+	     (let remaining_blocks = Seq.slice all_blocks n_blocks (Seq.length all_blocks) in
+	      contains_all_cipher_blocks x len remaining_len cipher remaining_blocks)))
+	(decreases (v remaining_len))
+#reset-options "--z3timeout 200 --initial_fuel 1 --max_fuel 1 --initial_ifuel 1 --max_ifuel 1"
+let rec counterblocks_contains_all_cipher_blocks i rgn x len remaining_len plain cipher = 
+  let x0 = {x with ctr=ctr_0 i +^ 1ul} in
+  let all_blocks = counterblocks i rgn x0 (v len) 0 (v len) plain cipher in
+  let completed_len = v x0.ctr - v (offset i) in
+  if remaining_len = 0ul then 
+    counterblocks_len rgn x0 (v len) 0 plain cipher
+  else let l = min remaining_len (PRF.blocklen i) in 
+       counterblocks_contains_all_cipher_blocks i rgn (PRF.incr i x) len (remaining_len -^ l) plain cipher;
+       admit()
+  
+  assert (completed_len <= Seq.length all_blocks);
+  admit()
+  
+			     (rgn:region) -> 
+			     (x:domain i{ctr_0 i <^ x.ctr}) ->
+			     (len:nat{len <> 0}) ->
+			     (from_pos:nat{from_pos <= len /\ safelen i (len - from_pos) x.ctr}) ->
+			     (plain:Plain.plain i len) ->
+			     (cipher:lbytes len) ->
+
+let x0 = {x with ctr=ctr_0 i +^ 1ul} in
+	     	     
+  let x0 = 
+  
+   if remaining_len = 0ul then ()
+   else ()
+   let from_pos = len -^ remaining_len in
+        let to_pos = len in    
+       let l0 = minNat remaining blockl in 
+    let l_32 = UInt32.uint_to_t l0 in 
+    let plain_hd = Crypto.Plain.slice plain from_pos (from_pos + l0) in
+    let cipher_hd = Seq.slice cipher from_pos (from_pos + l0) in
+    let block = PRF.Entry x (PRF.OTP l_32 plain_hd cipher_hd) in
+    let blocks = counterblocks i rgn (PRF.incr i x) l (from_pos + l0) to_pos plain cipher in
+    SeqProperties.cons block blocks
+
+   
+
+  i:id {safeId i} -> 
+  rgn:region -> 
+  x:PRF.domain i{PRF.ctr_0 i <^ ctr x} -> 
+  len:u32{len <> 0ul /\ safelen i (v len) (PRF.ctr_0 i +^ 1ul)} ->
+  remaining_len:u32{safelen i (v remaining_len) x.ctr /\ remaining_len <=^ len} -> 
+  plain:Crypto.Plain.plain i (v len) -> 
+  cipher:lbytes (v len) -> 
+
+  Tot (Seq.seq (PRF.entry rgn i)) // each entry e {PRF(e.x.id = x.iv /\ e.x.ctr >= ctr x)}
+  (decreases (to_pos - from_pos))
+
+
+(i:id{safeId i}) ->
+					      (n:Cipher.iv (alg i)) ->
+					      (st:state i Reader) ->
+		      			      #aadlen:UInt32.t {aadlen <=^ aadmax} ->
+					      (aad:lbuffer (v aadlen)) ->
+					      #plainlen:UInt32.t {plainlen <> 0ul /\ safelen i (v plainlen) (PRF.ctr_0 i +^ 1ul)} ->
+					      (cipher_tagged:lbuffer (v plainlen + v MAC.taglen)) ->
+					      (p:plain i (v plainlen)) ->
+					      (entry:entry i) ->
+					      (blocks: prf_blocks st.prf.mac_rgn i) ->
+					      (h:mem{Buffer.live h cipher_tagged}) ->
 
 val intro_contains_all_cipher_blocks: (i:id{safeId i}) ->
 				      (n:Cipher.iv (alg i)) ->
